Classic HL

HL/VCG.thy
@@ -2,7 +2,6 @@ section {* Verification condition generator *}
 
 theory VCG
   imports While "$AFP/KAT_and_DRA/SingleSorted/KAT_Models" "$ISABELLE_HOME/src/HOL/Eisbach/Eisbach"
-  Heap
 begin
 
 no_notation comp_op ("n_" [90] 91)
@@ -19,27 +18,36 @@ text {* \emph{hoare} tactic *}
 
 named_theorems hl_rules
 
+(*
 method hoare_init uses simp = 
   ((rule allI | rule ballI | subst simp | subst fst_conv | subst snd_conv)+)?
+*)
+
+method hoare_init uses simp = 
+  ((subst simp | subst fst_conv | subst snd_conv)+)?
 
 method hoare_step uses simp hl = 
-  (hoare_init simp: simp, (assumption | rule subset_refl | rule hl hl_rules))
+  (hoare_init simp: simp, (assumption | rule subset_refl | rule mono_rules | rule hl hl_rules | rule allI | rule ballI))
 
 method hoare_ind uses simp hl = 
   (hoare_step simp: simp hl: hl; (hoare_ind simp: simp hl: hl)?)+
 
-method hoare uses simp first hl = 
-  (hoare_init; (rule first)?; (hoare_ind simp: simp hl: hl)?)
+method hoare uses simp hl = 
+  (hoare_init simp: simp; (hoare_ind simp: simp hl: hl)?)
+
+method hl_aux uses rule =
+  (rule allI, rule rule; ((erule_tac x=u in allE)+, assumption))
+  
 
 (***********************************************************************************************)
 
 text {* Classic Hoare logic *}
 
-definition ht :: "'a set \<Rightarrow> 'a option rel \<Rightarrow> 'a set \<Rightarrow> bool" where
+definition ht :: "'a set \<Rightarrow> 'a rel \<Rightarrow> 'a set \<Rightarrow> bool" where
   "ht P x Q \<equiv> \<lfloor>P\<rfloor>;x \<subseteq> x;\<lfloor>Q\<rfloor>"
 
 lemma ht_true: "ht P x UNIV"
-  oops
+  by (auto simp: ht_def seq_def)
 
 lemma hl_false [intro]: "ht {} x Q"
   by (auto simp: ht_def seq_def test_def)
@@ -50,37 +58,37 @@ lemma hl_abort [hl_rules]: "ht P abort Q"
 lemma hl_skip [hl_rules]: "P \<subseteq> Q \<Longrightarrow> ht P skip Q"
   by (auto simp: ht_def skip_def seq_def test_def)
   
-lemma hl_graph [hl_rules]: "P \<subseteq> {s. case f (Some s) of None \<Rightarrow> False | Some q \<Rightarrow> q \<in> Q} \<Longrightarrow> ht P (graph f) Q"
-  apply (auto simp: ht_def graph_def seq_def test_def)
-apply (rule relcompI)
-apply auto
-by (metis (no_types, lifting) Ball_Collect case_optionE)
+lemma hl_graph [hl_rules]: "P \<subseteq> {s. f s \<in> Q} \<Longrightarrow> ht P (graph f) Q"
+  by (auto simp: ht_def graph_def seq_def test_def)
 
 lemma hl_assign [hl_rules]: "P \<subseteq> subst Q z_upd t \<Longrightarrow> ht P (assign z_upd t) Q"
+  by (auto simp: assign_def subst_def intro!: hl_graph)
+
+lemma hl_assign_aux [hl_rules]: "\<forall>z. P z \<subseteq> subst (Q z) z_upd t \<Longrightarrow> \<forall>z. ht (P z) (assign z_upd t) (Q z)"
   by (auto simp: assign_def subst_def intro!: hl_graph)
 
 lemma hl_seq [hl_rules]: "ht R y Q \<Longrightarrow> ht P x R \<Longrightarrow> ht P (x; y) Q"
   by (force simp: ht_def seq_def)
 
+lemma hl_seq_aux [hl_rules]: "\<forall>u. ht (R u) (y u) (Q u) \<Longrightarrow> \<forall>u. ht (P u) (x u) (R u) \<Longrightarrow> \<forall>u. ht (P u) (x u; y u) (Q u)"
+  by (hl_aux rule: hl_seq)
+
 lemma hl_split: "ht P x {t. Q t} \<Longrightarrow> ht P x {t. Q' t} \<Longrightarrow> ht P x {t. Q t \<and> Q' t}"
   by (force simp: ht_def seq_def test_def)
- 
-definition to_test :: "('a, 'b) pred \<Rightarrow> ('a, 'b) state set" where
-  "to_test P \<equiv> {<p> | p. p \<in> P}"
 
-lemma hl_cond : "ht (b \<sqinter> P) x Q \<Longrightarrow> ht (-b \<sqinter> P) y Q \<Longrightarrow> ht P (cond (to_test b) x y) Q"
-sorry(*
-  apply (auto simp: ht_def cond_def seq_def to_test_def test_def)
-*)
+lemma hl_split_aux: "\<forall>u. ht (P u) x {t. (Q u) t} \<Longrightarrow> \<forall>u. ht (P u) x {t. Q' u t} \<Longrightarrow> \<forall>u. ht (P u) x {t. Q u t \<and> Q' u t}"
+  by (hl_aux rule: hl_split)
 
-lemma hl_cond_aux [hl_rules]: "P \<subseteq> (P' \<union> - b) \<inter> (P'' \<union> b)  \<Longrightarrow> ht P' x Q \<Longrightarrow> ht P'' y Q \<Longrightarrow> ht P (cond (to_test b) x y) Q"
-sorry (*
+lemma hl_cassic_cond : "ht (b \<sqinter> P) x Q \<Longrightarrow> ht (-b \<sqinter> P) y Q \<Longrightarrow> ht P (cond b x y) Q"
+  by (fastforce simp: ht_def cond_def seq_def test_def)
+
+lemma hl_cond [hl_rules]: "P \<subseteq> (P' \<union> - b) \<inter> (P'' \<union> b)  \<Longrightarrow> ht P' x Q \<Longrightarrow> ht P'' y Q \<Longrightarrow> ht P (cond b x y) Q"
   by (fastforce simp: ht_def cond_def seq_def)
-*)
 
-lemma hl_while: "ht (b \<sqinter> i) x i \<Longrightarrow> ht i (cwhile (to_test b) x) (-b \<sqinter> i)"
-sorry
-(*
+lemma hl_cond_aux [hl_rules]: "\<forall>u. P u \<subseteq> (P' u \<union> - b) \<inter> (P'' u \<union> b)  \<Longrightarrow> \<forall>u. ht (P' u) x (Q u) \<Longrightarrow> \<forall>u. ht (P'' u) y (Q u) \<Longrightarrow> \<forall>u. ht (P u) (cond b x y) (Q u)"
+  by (hl_aux rule: hl_cond)
+
+lemma hl_while: "ht (b \<sqinter> i) x i \<Longrightarrow> ht i (cwhile b x) (-b \<sqinter> i)"
 proof (simp add: ht_def cwhile_def seq_def)
   assume "\<lfloor>b \<sqinter> i\<rfloor> O x \<subseteq> x O \<lfloor>i\<rfloor>"
   hence "\<lfloor>i\<rfloor> O (\<lfloor>b\<rfloor> O x)\<^sup>* \<subseteq> (\<lfloor>b\<rfloor> O x)\<^sup>* O \<lfloor>i\<rfloor>"
@@ -88,7 +96,6 @@ proof (simp add: ht_def cwhile_def seq_def)
   thus "\<lfloor>i\<rfloor> O (\<lfloor>b\<rfloor> O x)\<^sup>* O \<lfloor>-b\<rfloor> \<subseteq> ((\<lfloor>b\<rfloor> O x)\<^sup>* O \<lfloor>-b\<rfloor>) O \<lfloor>-b \<sqinter> i\<rfloor>"
     by auto
 qed
-*)
 
 (***********************************************************************************************)
 
@@ -98,38 +105,36 @@ lemma hl_pre: "P \<le> P' \<Longrightarrow> ht P' x Q \<Longrightarrow> ht P x Q
   by (fastforce simp: ht_def le_fun_def seq_def test_def)
 
 lemma hl_post: "Q' \<le> Q \<Longrightarrow> ht P x Q' \<Longrightarrow> ht P x Q"
-sorry
-(*
   by (fastforce simp: ht_def le_fun_def seq_def test_def)
-*)
+
+lemma hl_post_aux: "\<forall>u. Q' u \<le> Q u \<Longrightarrow> \<forall>u. ht (P u) x (Q' u) \<Longrightarrow> \<forall>u. ht (P u) x (Q u)"
+  by (fastforce simp: ht_def le_fun_def seq_def test_def)
+
 lemma hl_classic: "P \<le> P' \<Longrightarrow> Q' \<le> Q \<Longrightarrow> ht P' x Q' \<Longrightarrow> ht P x Q"
-sorry
-(*
-  by (fastforce simp: ht_def le_fun_def seq_def )
-*)
+  by (fastforce simp: ht_def le_fun_def seq_def)
   
 lemma hl_conseq: "\<forall>z. ht (P' z) c (Q' z) \<Longrightarrow> \<forall>s. s \<in> P \<longrightarrow> (\<exists>z. s \<in> P' z \<and> (Q' z \<subseteq> Q)) \<Longrightarrow> ht P c Q"
-sorry (*
-  by (force simp: ht_def seq_def )
-*)
-lemma hl_kleymann: "\<forall>z. ht (P' z) x (Q' z) \<Longrightarrow> \<forall>s t. (\<forall>z. s \<in> P' z \<longrightarrow> t \<in> Q' z) \<longrightarrow> (\<forall>z. s \<in> P z \<longrightarrow> t \<in> Q z) \<Longrightarrow> \<forall>z. ht (P z) x (Q z)"
- sorry
-(*
+  by (force simp: ht_def seq_def)
+
+lemma hl_kleymann: "\<forall>z. ht (P' z) x (Q' z) \<Longrightarrow> \<forall>s t. (\<forall>z. s \<in> P' z \<longrightarrow> t \<in> Q' z) \<longrightarrow> (\<forall>z. s \<in> P z \<longrightarrow> t \<in> Q z) \<Longrightarrow> ht (P z) x (Q z)"
  by (fastforce simp: apre_def seq_def ht_def)
-*)
-(*
+
+lemma hl_kleymann_aux: "\<forall>z. ht (P' z) x (Q' z) \<Longrightarrow> \<forall>s t. (\<forall>z. s \<in> P' z \<longrightarrow> t \<in> Q' z) \<longrightarrow> (\<forall>z. s \<in> P z \<longrightarrow> t \<in> Q z) \<Longrightarrow> \<forall>z. ht (P z) x (Q z)"
+ by (hl_aux rule: hl_kleymann)
+
 lemma hl_for [hl_rules]: "\<forall>s. m_upd(\<lambda>_. m s) s = s \<Longrightarrow> 
   ht P (assign j_upd n) (subst Q m_upd j \<inter> {s. j s \<le> m s}) \<Longrightarrow> 
   ht ({s. j s < m s} \<inter> subst Q m_upd j) x (subst (subst Q m_upd j \<inter> {s. j s \<le> m s}) j_upd (\<lambda>s. j s + 1)) \<Longrightarrow> 
   ht P (cfor (j_upd, j) n (m_upd, m) x) Q"
-  apply (hoare simp: cfor_def first: hl_post [where Q'="(-{s. j s < m s} \<inter> (subst Q m_upd j \<inter> {s. j s \<le> m s}))"] hl: hl_while)
+  apply (rule hl_post [where Q'="(-{s. j s < m s} \<inter> (subst Q m_upd j \<inter> {s. j s \<le> m s}))"])
   apply (subgoal_tac "-{s. j s < m s} \<inter> (subst Q m_upd j \<inter> {s. j s \<le> m s}) = {s. j s = m s} \<inter> subst Q m_upd j")
   apply (force simp: subst_def)
   apply force
+  apply (hoare simp: cfor_def hl: hl_while)
   apply (subgoal_tac "{s. j s < m s} \<inter> (subst Q m_upd j \<inter> {s. j s \<le> m s}) = {s. j s < m s} \<inter> subst Q m_upd j")
   apply force+
 done
-*)
+
 (***********************************************************************************************)
 
 text {* Blocks / Procedures / Recursive Calls *}
@@ -138,13 +143,11 @@ text {* Blocks / Procedures / Recursive Calls *}
 lemma hl_dyn [hl_rules]: "\<forall>s \<in> P. ht P (g s) Q \<Longrightarrow> ht P (\<lceil>g\<rceil>) Q"
   by (fastforce simp: ht_def seq_def dyn_def)
 
-(*
-lemma hl_local_inv: "\<forall>s s'. z (z_upd (\<lambda>_. z s) s') = z s \<Longrightarrow> P \<le> {(s, h). z s = u} \<Longrightarrow> ht P (loc_block (z_upd, z) t x) {(s, h). z s = u}"
+lemma hl_local_inv: "\<forall>s s'. z (z_upd (\<lambda>_. z s) s') = z s \<Longrightarrow> P \<le> {s. z s = u} \<Longrightarrow> ht P (loc_block (z_upd, z) t x) {s. z s = u}"
   by (auto simp: block_def loc_block_def graph_def dyn_def seq_def ht_def)
-*)
-(*
+
 lemma hl_block: "\<forall>s. ht P x {t. f s t \<in> Q} \<Longrightarrow> ht P (block x f) Q"
-  by (hoare simp: block_def) force
+  by (hoare simp: block_def hl: ballI) force
 
 lemma hl_loc_block: "\<forall>s. ht P (\<langle>\<lambda>s. z_upd (\<lambda>_. t s) s\<rangle>; x) {t. z_upd s t \<in> Q} \<Longrightarrow> ht P (loc_block (z_upd, z) t x) Q"
   by (auto simp: loc_block_def intro: hl_block)
@@ -154,59 +157,71 @@ lemma hl_fun_block_inv: "\<forall>s s'. y (y_upd (\<lambda>_. y s) s') = y s \<L
 
 lemma hl_fun_block: "\<forall>s. ht P R {t. y_upd (\<lambda>_. y s) (z_upd (\<lambda>_. y t) t) \<in> Q} \<Longrightarrow> ht P (fun_call z_upd (R, (y_upd, y))) Q"
   by (auto simp: fun_call_def intro: hl_block)
-*)
-lemma hl_Sup: "\<forall>x \<in> X. \<forall>z. ht (P z) (x z) (Q z) \<Longrightarrow> \<forall>z. ht (P z) (Sup X z) (Q z)"
-sorry (*
-  by (fastforce simp: ht_def seq_def)
-*)
 
-lemma hl_rec [hl_rules]: "mono f \<Longrightarrow> (\<And>x. \<forall>z. ht (P z) (x z) (Q z) \<Longrightarrow> \<forall>z. ht (P z) (f x z) (Q z)) \<Longrightarrow> \<forall>z. ht (P z) (lfp f z) (Q z)"
-  apply (erule lfp_ordinal_induct [where f=f], simp)
+lemma hl_Sup: "\<forall>x \<in> X. \<forall>z. ht (P z) (x z) (Q z) \<Longrightarrow> \<forall>z. ht (P z) (Sup X z) (Q z)"
+  by (fastforce simp: ht_def seq_def)
+
+lemma hl_rec_dep: "mono f \<Longrightarrow> (\<And>x. \<forall>z. ht (P z) (x z) (Q z) \<Longrightarrow> \<forall>z. ht (P z) (f x z) (Q z)) \<Longrightarrow> \<forall>z. ht (P z) (lfp f z) (Q z)"
+  apply (erule lfp_ordinal_induct [where f=f], assumption)
   by (force intro!: hl_Sup)
 
-(***********************************************************************************************)
+lemma hl_rec_aux [hl_rules]: "mono f \<Longrightarrow> (\<And>x. \<forall>z. ht (P z) x (Q z) \<Longrightarrow> \<forall>z. ht (P z) (f x) (Q z)) \<Longrightarrow> \<forall>z. ht (P z) (lfp f) (Q z)"
+  apply (erule lfp_ordinal_induct [where f=f], simp)
+  by (fastforce simp: ht_def seq_def)
 
-text {* Frame rule -- Separation logic *}
-
-no_notation times (infixl "*" 70)
-(*
-lemma "local x \<Longrightarrow> ht p x q \<Longrightarrow> ht (p * r) x (q * r)"
-  apply (auto simp: ht_def local_def sep_conj_def)
-  *)
+lemma hl_rec [hl_rules]: "mono f \<Longrightarrow> (\<And>x. \<forall>z. ht (P z) x (Q z) \<Longrightarrow> \<forall>z. ht (P z) (f x) (Q z)) \<Longrightarrow> ht (P z) (lfp f) (Q z)"
+  apply (drule hl_rec_aux)
+prefer 2
+  apply (erule_tac x=z in allE)
+  apply assumption
+apply simp
+done
 
 (***********************************************************************************************)
 
 text {* Annotated programs *}
 
 lemma hl_awhile [hl_rules]: "P \<subseteq> i \<Longrightarrow> -b \<inter> i \<subseteq> Q \<Longrightarrow> ht (b \<sqinter> i) x i \<Longrightarrow> ht P (awhile i b x) Q"
-  by (hoare simp: awhile_def first: hl_conseq hl: hl_while) force
+  apply (rule hl_conseq)
+  by (hoare simp: awhile_def hl: allI hl_while) force
   
 lemma hl_apre_classic: "P \<le> P' \<Longrightarrow> ht P' x Q \<Longrightarrow> ht P (apre P' x) Q"
-  by (hoare simp: apre_def first: hl_pre)
+  apply (rule hl_pre, assumption)
+  by (hoare simp: apre_def)
 
-lemma hl_apre_kleymann_aux: "\<forall>z. ht (P' z) x (Q z) \<Longrightarrow> \<forall>s t. (\<forall>z. s \<in> P' z \<longrightarrow> t \<in> Q z) \<longrightarrow> (\<forall>z. s \<in> P z \<longrightarrow> t \<in> Q z) \<Longrightarrow> \<forall>z. ht (P z) (apre (P' z) x) (Q z)"
+lemma hl_apre_kleymann [hl_rules]: "ht P' x Q' \<Longrightarrow> \<forall>s t. (s \<in> P' \<longrightarrow> t \<in> Q') \<longrightarrow> (s \<in> P \<longrightarrow> t \<in> Q) \<Longrightarrow> ht P (apre P x) Q"
   by (force simp add: apre_def seq_def ht_def)
 
-lemma hl_apre_kleymann: "ht P' x Q \<Longrightarrow> \<forall>s t. (s \<in> P' \<longrightarrow> t \<in> Q) \<longrightarrow> (s \<in> P \<longrightarrow> t \<in> Q) \<Longrightarrow> ht P (apre P' x) Q"
-  by (force simp add: apre_def seq_def ht_def)
-                                                                               
+lemma hl_apre_kleymann_aux [hl_rules]: "\<forall>z. ht (P' z) x (Q' z) \<Longrightarrow> \<forall>s t. (\<forall>z. s \<in> P' z \<longrightarrow> t \<in> Q' z) \<longrightarrow> (\<forall>z. s \<in> P z \<longrightarrow> t \<in> Q z) \<Longrightarrow> \<forall>z. ht (P z) (apre_aux P x) (Q z)"
+  by (force simp add: apre_aux_def seq_def ht_def)
+                                                                 
 lemma hl_apost_classic [hl_rules]: "Q' \<le> Q \<Longrightarrow> ht P x Q' \<Longrightarrow> ht P (apost x Q') Q"
   by (hoare simp: apost_def hl: hl_apre_kleymann) force
   
 lemma hl_aprog_classic : "P \<le> P' \<Longrightarrow> Q' \<le> Q \<Longrightarrow> ht P' x Q' \<Longrightarrow> ht P (aprog P' x Q') Q"
-  by (hoare simp: aprog_def first: hl_classic)
+  apply (rule hl_classic, assumption+)
+  by (hoare simp: aprog_def)
+
+lemma hl_aprog_kleymann_aux [hl_rules]: "\<forall>z. ht (P' z) x (Q' z) \<Longrightarrow> \<forall>s t. (\<forall>z. s \<in> P' z \<longrightarrow> t \<in> Q' z) \<longrightarrow> (\<forall>z. s \<in> P z \<longrightarrow> t \<in> Q z) \<Longrightarrow> \<forall>z. Q z \<le> Q'' z \<Longrightarrow> \<forall>z. ht (P z) (aprog_aux P x Q) (Q'' z)"
+  apply (simp add: aprog_aux_def)
+  apply (rule hl_post_aux)
+  apply assumption
+  by (force simp add: aprog_aux_def seq_def ht_def)
 
 (***********************************************************************************************)
 
 text {* When using hoare, rules should be applied in the following order *}
-(*
+
 declare 
   hl_local_inv [hl_rules]
   hl_loc_block [hl_rules]
   hl_fun_block_inv [hl_rules]
   hl_fun_block [hl_rules]
   hl_block [hl_rules]
-*)
+
 declare subst_def [simp]
-  and case_optionE [elim!]
+
+method hoare_split uses simp hl = 
+  (hoare_init simp: simp; (rule hl_split)+; (hoare_ind simp: simp hl: hl)?)
+
 end
