Heap.thy
@@ -28,8 +28,8 @@ interpretation heap?: locality "op ++" "op \<bottom>" Map.empty
 
 section {* Commands *}
 
-lemma local_skip: "Local \<lbrakk>skip\<rbrakk>"
-  by (auto simp: Local_def skip_def ptran_def)
+lemma local_skip: "local \<langle>skip\<rangle>"
+  by (auto simp: local_def skip_def stran_def)
 
 lemma safe_skip: "safe skip"
   by (simp add: Local_local local_safe local_skip)
@@ -37,11 +37,11 @@ lemma safe_skip: "safe skip"
 lemma frame_skip: "frame skip"
   by (simp add: Local_local local_frame local_skip)
 
-definition lookup :: "(nat, 'a) lval \<Rightarrow> ('a \<Rightarrow> nat) \<Rightarrow> ('a, 'b) state rel" where
-  "lookup u_upd t \<equiv> \<langle>\<lambda>\<sigma>. case \<sigma> of Some (s, h) \<Rightarrow> if t s \<in> dom h then Some (u_upd (\<lambda>_. the (h (t s))) s, h) else None | None \<Rightarrow> None\<rangle>"
+definition lookup :: "(nat, 'a) lval \<Rightarrow> ('a \<Rightarrow> nat) \<Rightarrow> ('a, heap) state rel" where
+  "lookup u_upd t \<equiv> \<langle>\<lambda>\<sigma>. case \<sigma> of <s, h> \<Rightarrow> if t s \<in> dom h then <u_upd (\<lambda>_. the (h (t s))) s, h> else fault | fault \<Rightarrow> fault\<rangle>"
 
-definition mutation :: "('a \<Rightarrow> nat) \<Rightarrow> ('a \<Rightarrow> nat) \<Rightarrow> ('a, 'b) state rel" where
-  "mutation u t \<equiv> \<langle>\<lambda>\<sigma>. case \<sigma> of Some (s, h) \<Rightarrow> if u s \<in> dom h then Some (s, h(u s \<mapsto> t s)) else None | None \<Rightarrow> None\<rangle>"
+definition mutation :: "('a \<Rightarrow> nat) \<Rightarrow> ('a \<Rightarrow> nat) \<Rightarrow> ('a, heap) state rel" where
+  "mutation u t \<equiv> \<langle>\<lambda>\<sigma>. case \<sigma> of <s, h> \<Rightarrow> if u s \<in> dom h then <s, h(u s \<mapsto> t s)> else fault | fault \<Rightarrow> fault\<rangle>"
 
 lemma "safe (assign u_upd t)"
   by (auto simp add: safe_def assign_def graph_def)
@@ -50,17 +50,24 @@ lemma "frame (assign u_upd t)"
   by (auto simp add: frame_def assign_def graph_def)
 
 lemma "safe (lookup u_upd t)"
-  by (auto simp add: safe_def lookup_def graph_def partial_semigroup_class.pleq_def)
+  by (auto simp add: safe_def lookup_def graph_def substate_def)
 
 lemma "frame (lookup u_upd t)"
   by (auto simp add: frame_def lookup_def graph_def)
 
 lemma "safe (mutation u_upd t)"
-  by (auto simp add: safe_def mutation_def graph_def partial_semigroup_class.pleq_def)
+  by (auto simp add: safe_def mutation_def graph_def substate_def)
 
 lemma "frame (mutation u_upd t)"
   apply (clarsimp simp add: frame_def mutation_def graph_def ortho_def)
   by (metis disjoint_iff_not_equal domI map_add_upd_left)
 
+lemma "safe (assign u_upt t)"
+  by (auto simp: assign_def safe_def graph_def)
 
+lemma "frame (assign u_upt t)"
+  by (auto simp: assign_def frame_def graph_def)
+
+
+no_notation heap.stran ("\<langle>_\<rangle>")
 end
