Algebra/RKAT.thy
@@ -3,89 +3,103 @@ theory RKAT
 begin
 
 class rkat = kat +
-  fixes spec_op :: "'a \<Rightarrow> 'a \<Rightarrow> 'a" (":[_ _]" [50,50] 100)
-  assumes spec_def: "test p \<Longrightarrow> test q \<Longrightarrow> p\<cdot>x \<le> x\<cdot>q \<longleftrightarrow> x \<le> :[p q]"
+  fixes spec :: "'a \<Rightarrow> 'a \<Rightarrow> 'a"
+  assumes spec_def: "test p \<Longrightarrow> test q \<Longrightarrow> p\<cdot>x \<le> x\<cdot>q \<longleftrightarrow> x \<le> spec p q"
 begin
 
 definition ref_order :: "'a \<Rightarrow> 'a \<Rightarrow> bool" (infix "\<sqsubseteq>" 50) where
   "x \<sqsubseteq> y \<equiv> y \<le> x"
 
-lemma spec_char: "test p \<Longrightarrow> test q \<Longrightarrow> p\<cdot>:[p q] \<le> :[p q]\<cdot>q"
-  by (metis eq_refl spec_def)
+lemma ref_order_refl [simp]: "spec p q \<sqsubseteq> spec p q"
+  by (auto simp: ref_order_def)
 
-lemma specI [intro]: "test p \<Longrightarrow> test q \<Longrightarrow> p\<cdot>x \<le> x\<cdot>q \<Longrightarrow> :[p q] \<sqsubseteq> x"
+lemma spec_char [simp]: "test p \<Longrightarrow> test q \<Longrightarrow> p\<cdot>(spec p q) \<le> (spec p q)\<cdot>q"
+  by (simp add: spec_def)
+
+lemma specI [intro]: "test p \<Longrightarrow> test q \<Longrightarrow> p\<cdot>x \<le> x\<cdot>q \<Longrightarrow> (spec p q) \<sqsubseteq> x"
   by (simp add: spec_def ref_order_def)
 
-lemma spec_mult_isol: "x \<sqsubseteq> y \<Longrightarrow> z\<cdot>x \<sqsubseteq> z\<cdot>y"
+lemma spec_mult_isol [intro]: "x \<sqsubseteq> y \<Longrightarrow> z\<cdot>x \<sqsubseteq> z\<cdot>y"
   by (simp add: mult_isol ref_order_def)
 
-lemma spec_mult_isor: "x \<sqsubseteq> y \<Longrightarrow> x\<cdot>z \<sqsubseteq> y\<cdot>z"
+lemma spec_mult_isor [intro]: "x \<sqsubseteq> y \<Longrightarrow> x\<cdot>z \<sqsubseteq> y\<cdot>z"
   by (simp add: mult_isor ref_order_def)
 
-lemma star_iso: "x \<sqsubseteq> y \<Longrightarrow> x\<^sup>\<star> \<sqsubseteq> y\<^sup>\<star>"
+lemma star_iso [intro]: "x \<sqsubseteq> y \<Longrightarrow> x\<^sup>\<star> \<sqsubseteq> y\<^sup>\<star>"
   by (simp add: star_iso ref_order_def)
 
 lemma ref_order_trans [trans]: "x \<sqsubseteq> y \<Longrightarrow> y \<sqsubseteq> z \<Longrightarrow> x \<sqsubseteq> z"
   by (simp add: ref_order_def)
 
-lemma strengthen_post: "\<lbrakk>test p; test q; test q'\<rbrakk> \<Longrightarrow> q' \<le> q \<Longrightarrow> :[p q] \<sqsubseteq> :[p q']"
+lemma strengthen_post [intro]: "test p \<Longrightarrow> test q \<Longrightarrow> test q' \<Longrightarrow> q' \<le> q \<Longrightarrow> spec p q \<sqsubseteq> spec p q'"
   by (meson specI local.mult_isol local.order_trans spec_char)
 
-lemma weaken_pre: "\<lbrakk>test p; test p'; test q\<rbrakk> \<Longrightarrow> p \<le> p' \<Longrightarrow> :[p q] \<sqsubseteq> :[p' q]"
+lemma weaken_pre [intro]: "test p \<Longrightarrow> test q \<Longrightarrow> test p' \<Longrightarrow> p \<le> p' \<Longrightarrow> spec p q \<sqsubseteq> spec p' q"
   by (meson specI local.mult_isor local.order_trans spec_char)
 
-lemma weaken_and_strengthen: "\<lbrakk>test p; test p'; test q; test q'\<rbrakk> \<Longrightarrow> p \<le> p' \<Longrightarrow> q' \<le> q \<Longrightarrow> :[p q] \<sqsubseteq> :[p' q']"
+lemma weaken_and_strengthen [intro]: "test p \<Longrightarrow> test q \<Longrightarrow> test p' \<Longrightarrow> test q' \<Longrightarrow> p \<le> p' \<Longrightarrow> q' \<le> q \<Longrightarrow> spec p q \<sqsubseteq> spec p' q'"
   by (metis ref_order_trans strengthen_post weaken_pre)
 
-lemma skip_ref: ":[1 1] \<sqsubseteq> 1"
+lemma skip_ref [simp]: "spec 1 1 \<sqsubseteq> 1"
   using local.test_one_var by blast
 
-lemma abort_ref: ":[0 1] \<sqsubseteq> x"
+lemma abort_ref [simp]: "spec 0 1 \<sqsubseteq> x"
   using local.test_one_var local.test_zero_var by auto
 
-lemma magic_ref: "x \<sqsubseteq> :[1 0]"
-  using local.spec_def local.test_one_var local.test_zero_var ref_order_def by force
+lemma magic_ref [simp]: "x \<sqsubseteq> spec 1 0"
+  by (metis local.annir local.mult_1_left local.zero_least local.zero_unique ref_order_def spec_char test_one_var test_zero_var)
 
-lemma magic_eq_zero [simp]: ":[1 0] = 0"
+lemma magic_eq_zero [simp]: "spec 1 0 = 0"
   using local.zero_unique magic_ref ref_order_def by blast
 
-lemma skip_ref_var1: "test p \<Longrightarrow> :[p 1] \<sqsubseteq> 1"
+lemma skip_ref_var1: "test p \<Longrightarrow> spec p 1 \<sqsubseteq> 1"
   by (auto simp: test_one_var local.test_ub_var)
 
-lemma skip_ref_var2 [intro!]: "\<lbrakk>test p; test q; p \<le> q\<rbrakk> \<Longrightarrow> :[p q] \<sqsubseteq> 1"
+lemma skip_ref_var2 [intro!]: "test p \<Longrightarrow> test q \<Longrightarrow> p \<le> q \<Longrightarrow> spec p q \<sqsubseteq> 1"
   by auto
 
-lemma sequence_ref [intro]: "\<lbrakk>test p; test q; test r\<rbrakk> \<Longrightarrow> :[p q] \<sqsubseteq> :[p r] \<cdot> :[r q]"
+lemma sequence_ref [intro]: "test p \<Longrightarrow> test q \<Longrightarrow> test r \<Longrightarrow> spec p q \<sqsubseteq> (spec p r) \<cdot> (spec r q)"
 proof -
   assume hyp: "test p" "test q" "test r"
-  hence "p \<cdot> :[p r] \<cdot> :[r q] \<le> :[p r] \<cdot> r \<cdot> :[r q]"
-    by (simp add: local.mult_isor spec_char)
-  also have "... \<le> :[p r] \<cdot> :[r q] \<cdot> q"
-    by (simp add: hyp local.mult_isol mult_assoc spec_char)
+  hence "p \<cdot> (spec p r) \<cdot> (spec r q) \<le> (spec p r) \<cdot> r \<cdot> (spec r q)"
+    by (simp add: local.mult_isor)
+  also have "... \<le> (spec p r) \<cdot> (spec r q) \<cdot> q"
+    by (simp add: hyp local.mult_isol mult_assoc)
   finally show ?thesis
     by (auto simp: hyp mult_assoc)
 qed
 
-lemma choice_ref [intro]: ":[p q] \<sqsubseteq> x \<Longrightarrow> :[p q] \<sqsubseteq> y \<Longrightarrow> :[p q] \<sqsubseteq> x + y"
+lemma choice_ref [intro]: "test p \<Longrightarrow> test q \<Longrightarrow> spec p q \<sqsubseteq> x \<Longrightarrow> spec p q \<sqsubseteq> y \<Longrightarrow> spec p q \<sqsubseteq> x + y"
   by (simp add: local.add_lub ref_order_def)
 
-lemma test1_ref: "\<lbrakk>test b; test p; test q\<rbrakk> \<Longrightarrow> :[p q] \<sqsubseteq>  b\<cdot>:[p\<cdot>b q]"
-  by (metis local.test_eq3 local.test_mult_closed mult_assoc specI spec_char)
+lemma test_expl_ref: "test b \<Longrightarrow> test p \<Longrightarrow> test q \<Longrightarrow> spec p q \<sqsubseteq>  b \<cdot> (spec (p\<cdot>b) q)"
+  sorry
 
-lemma test2_ref: "\<lbrakk>test b; test p; test q\<rbrakk> \<Longrightarrow> :[p q\<cdot>b] \<sqsubseteq> :[p q] \<cdot> b"
+lemma test_expr_ref: "test b \<Longrightarrow> test p \<Longrightarrow> test q \<Longrightarrow> spec p (q\<cdot>b) \<sqsubseteq> (spec p q) \<cdot> b"
 oops
 
+lemma conditional_ref: "test b \<Longrightarrow> test p \<Longrightarrow> test q \<Longrightarrow> spec p q \<sqsubseteq>  b \<cdot> (spec (p\<cdot>b) q) + !b \<cdot> (spec (p\<cdot>!b) q)"
+  by (auto intro: test_expl_ref test_comp_closed)
+
+lemma while_ref: "test b \<Longrightarrow> test c \<Longrightarrow> test p \<Longrightarrow> spec p (p\<cdot>c) \<sqsubseteq> (b \<cdot> (spec (p\<cdot>b) p))\<^sup>\<star>\<cdot>c"
+  apply (auto intro!: specI)
+  apply (simp add: local.test_comp_closed_var local.test_mult_closed)
+  apply (subst mult_assoc[symmetric]) back
+  apply (subst mult_assoc)
+  apply (subst test_mult_comm_var) back back back back back back back
+  apply (simp add: test_comp_closed)
+  apply simp
+  apply (subst mult_assoc[symmetric]) back
+  apply (subst mult_assoc) back
+  apply (subst test_mult_idem_var)
+  apply (simp add: test_comp_closed)
+  apply (subst mult_assoc[symmetric])
+  apply (rule mult_isor[THEN impE])
+  prefer 2
+  apply assumption
+  apply (rule star_sim2)
+using local.spec_def ref_order_def test_expl_ref by auto
   
-lemma conditional_ref: "\<lbrakk>test b; test p; test q\<rbrakk> \<Longrightarrow> :[p q] \<sqsubseteq>  b\<cdot>:[p\<cdot>b q] + !b\<cdot>:[p\<cdot>!b q]"
-  by (auto intro: test_ref test_comp_closed)
-
-lemma while_ref: "\<lbrakk>test b; test p\<rbrakk> \<Longrightarrow> :[p p\<cdot>!b] \<sqsubseteq> (b\<cdot>:[p\<cdot>b p])\<^sup>\<star>\<cdot>!b"
-  apply (auto intro: specI)
-  by (metis hoare_triple_def_var spec_char1 spec_def test_mult_closed  while_rule)
-
-lemma ref_order_sym [simp]: ":[p q] \<sqsubseteq> :[p q]"
-  by (metis eq_refl)
-
 end
 
 end
