HL/BinSearch.thy
@@ -1,0 +1,96 @@
+theory BinSearch
+  imports Array Syntax
+begin
+
+no_notation Set.image (infixr "`" 90)
+
+hide_const first last sorted 
+
+hide_const last
+
+
+definition sorted :: "'a :: linorder array \<Rightarrow> nat \<Rightarrow> nat \<Rightarrow> bool" where
+  "sorted a i j \<equiv> \<forall>x y. i \<le> x \<and> x \<le> y \<and> y \<le> j \<longrightarrow> a<x> \<le> a<y>"
+
+
+lemma sorted_section1: "sorted a f l \<Longrightarrow> f \<le> m \<Longrightarrow> m < l \<Longrightarrow> a<m> < v \<Longrightarrow> (\<exists>x \<in>\<lbrace>f, l\<rbrace>. a<x> = v) \<longleftrightarrow> (\<exists>x \<in> \<lbrace>Suc m, l\<rbrace>. a<x> = v)"
+  apply (auto simp: sorted_def interval_def)
+  apply (metis leD less_imp_le_nat not_less_eq_eq)
+  apply (rule_tac x=x in exI)
+  apply clarsimp
+done
+
+lemma sorted_section2: "sorted a f l \<Longrightarrow> f \<le> m \<Longrightarrow> m \<le> l \<Longrightarrow> v \<le> a<m> \<Longrightarrow> (\<exists>x \<in> \<lbrace>f, l\<rbrace>. a<x> = v) \<longleftrightarrow> (\<exists>x \<in> \<lbrace>f, m\<rbrace>. a<x> = v)"
+  apply (auto simp: sorted_def interval_def)
+  by (meson eq_iff nat_le_linear)
+
+record state =
+  first :: nat
+  mid :: nat
+  last :: nat
+
+abbreviation f :: "nat \<times> nat \<Rightarrow> nat" where "f \<equiv> fst"
+abbreviation l :: "nat \<times> nat \<Rightarrow> nat" where "l \<equiv> snd"
+
+lemma "\<forall>u. \<turnstile> \<lbrace> (f u = `first \<and> l u = `last \<and> `first \<le> `last \<and> sorted a `first `last) \<rbrace>
+  rec BinSearch in 
+    `mid := (`first + `last) div 2;
+    if `first \<noteq> `last then
+      if a<`mid> < v then
+        `first := `mid + 1;
+        \<lbrace> u. (f u + l u) div 2 + 1 = `first \<and> l u = `last \<and> `first \<le> `last \<and> sorted a `first `last
+          \<and> sorted a (f u) (l u) \<and> a<(f u + l u) div 2> < v \<rbrace>
+        BinSearch
+        \<lbrace> (f u + l u) div 2 + 1 \<le> `mid \<and> `mid \<le> l u \<and> (a<`mid> = v \<longleftrightarrow> (\<exists>x \<in> \<lbrace>(f u + l u) div 2 + 1, l u\<rbrace>. a<x> = v))
+          \<and> sorted a (f u) (l u) \<and> a<(f u + l u) div 2> < v \<rbrace>
+      else 
+        if a<`mid> > v then
+          `last := `mid;
+          \<lbrace> u. (f u = `first \<and> (f u + l u) div 2 = `last \<and> `first \<le> `last \<and> sorted a `first `last 
+            \<and> sorted a (f u) (l u) \<and> v < a<(f u + l u) div 2> ) \<rbrace>
+          BinSearch
+          \<lbrace> f u \<le> `mid \<and> `mid \<le> (f u + l u) div 2 \<and> (a<`mid> = v \<longleftrightarrow> (\<exists>x \<in> \<lbrace>f u, (f u + l u) div 2\<rbrace>. a<x> = v))
+            \<and> sorted a (f u) (l u) \<and> v < a<(f u + l u) div 2> \<rbrace>
+        fi
+      fi
+    fi
+    end
+  \<lbrace> f u \<le> `mid \<and> `mid \<le> l u \<and> (a<`mid> = v \<longleftrightarrow> (\<exists>x \<in> \<lbrace>f u, l u\<rbrace>. a<x> = v)) \<rbrace>"
+apply hoare
+apply force
+
+apply clarsimp
+apply (rule conjI)
+apply force
+apply (subst sorted_section1) back
+apply assumption
+prefer 3
+apply assumption
+apply force
+apply force
+
+apply force
+
+apply force
+
+apply clarsimp
+apply (rule conjI)
+apply force
+apply (subst sorted_section2) back
+apply assumption
+apply assumption
+apply force
+
+defer
+
+defer
+
+apply clarsimp
+
+apply (auto simp: sorted_def interval_def)
+apply (rule_tac x="(first xa + last xa) div 2" in exI)
+apply force
+
+
+
+end
