HL/Refinement.thy
@@ -1,0 +1,120 @@
+theory Refinement
+  imports While "../../Algebra/RKAT_Models" "$ISABELLE_HOME/src/HOL/Eisbach/Eisbach"
+begin
+
+no_notation comp_op ("n_" [90] 91)
+  and test_operator  ("t_" [100] 101)
+  and floor ("\<lfloor>_\<rfloor>")
+  and ceiling ("\<lceil>_\<rceil>")
+  and Set.image (infixr "`" 90)
+  and rkat_class.ref_order (infix "\<sqsubseteq>" 50)
+
+abbreviation rel_ref_order (infix "\<sqsubseteq>" 50) where
+  "rel_ref_order \<equiv> rel_rkat.ref_order"
+
+abbreviation Spec :: "'a set \<Rightarrow> 'a set \<Rightarrow> 'a rel" where
+  "Spec P Q \<equiv> rel_spec (\<lfloor>P\<rfloor>) (\<lfloor>Q\<rfloor>)"
+
+lemma seq_assoc: "x; y; z = (x; y); z"
+  by (auto simp: seq_def)
+
+(***********************************************************************************************)
+
+text {* \emph{morgan} tactic *}
+
+named_theorems ref_rules
+
+method morgan_step uses simp ref = 
+  (assumption | rule ref ref_rules | subst seq_assoc)
+
+method morgan uses simp ref = 
+  (morgan_step simp: simp ref: ref; (morgan simp: simp ref: ref)?)+
+
+(***********************************************************************************************)
+
+text {* Remaining Morgan Refinement Laws *}
+
+lemma [simp]: "rel_dioid_tests.test (\<lfloor>P\<rfloor>)"
+  by (auto simp: rel_dioid_tests.test_def)
+
+lemma assignment_ref [intro]: "P \<subseteq> subst Q v m \<Longrightarrow> Spec P Q \<sqsubseteq> assign v m"
+  apply (clarsimp simp: subst_def assign_def rel_rkat.ref_order_def graph_def rel_spec_def)
+  apply (rule_tac x="{(s, v (\<lambda>_. m s) s)}" in exI, auto)
+done
+
+lemma following_assignment_ref: "Q' \<subseteq> subst Q v m \<Longrightarrow> Spec P Q \<sqsubseteq> Spec P Q'; assign v m"
+proof -
+  assume assms: "Q' \<subseteq> subst Q v m"
+  have "Spec P Q \<sqsubseteq> Spec P Q'; Spec Q' Q"
+    by (auto simp: seq_def)
+  also have "... \<sqsubseteq> Spec P Q'; assign v m"
+    using assms by (auto simp: seq_def)
+  finally show ?thesis .
+qed
+
+lemma leading_assignment_ref: "P \<subseteq> subst P' v m \<Longrightarrow> Spec P Q \<sqsubseteq> assign v m; Spec P' Q"
+proof -
+  assume assms: "P \<subseteq> subst P' v m"
+  have "Spec P Q \<sqsubseteq> Spec P P'; Spec P' Q"
+    by (auto simp: seq_def)
+  also have "... \<sqsubseteq> assign v m; Spec P' Q"
+    using assms by (auto simp: seq_def)
+  finally show ?thesis .
+qed
+
+(* Annotated while Specification *)
+
+lemma while_ref_tactic: "\<lbrakk>I \<inter> B \<subseteq> P'; P \<subseteq> I; I - B \<subseteq> Q\<rbrakk> \<Longrightarrow> Spec P Q \<sqsubseteq> cwhile B (Spec P' I)"
+proof -
+  have a: "\<lfloor>I - B\<rfloor> = \<lfloor>I\<rfloor> O \<lfloor>-B\<rfloor>" by force
+  have b: "\<lfloor>I \<inter> B\<rfloor> = \<lfloor>I\<rfloor> O \<lfloor>B\<rfloor>" by force
+  assume assms: "I \<inter> B \<subseteq> P'" "P \<subseteq> I" "I - B \<subseteq> Q"
+  hence "Spec P Q \<sqsubseteq> rel_spec (\<lfloor>I\<rfloor>) (\<lfloor>I - B\<rfloor>)"
+    by auto
+  also have "... \<sqsubseteq> (\<lfloor>B\<rfloor> O Spec (I \<inter> B) I)\<^sup>* O \<lfloor>- B\<rfloor>"
+    by (auto simp: a b intro: rel_rkat.while_ref)
+  also have "... \<sqsubseteq> (\<lfloor>B\<rfloor> O Spec P' I)\<^sup>* O \<lfloor>- B\<rfloor>"
+    using assms by force
+  finally show ?thesis
+    by (simp add: cwhile_def seq_def)
+qed
+                                       
+lemma while_iso: "c \<sqsubseteq> c' \<Longrightarrow> cwhile b c \<sqsubseteq> cwhile b c'"
+  by (auto simp: cwhile_def seq_def)
+
+lemma spec_mult_isol: "x \<sqsubseteq> y \<Longrightarrow> z; x \<sqsubseteq> z; y"
+  by (simp add: seq_def rel_rkat.spec_mult_isol)
+
+lemma spec_mult_isor: "x \<sqsubseteq> y \<Longrightarrow> x; z \<sqsubseteq> y; z"
+  by (simp add: seq_def rel_rkat.spec_mult_isor)
+
+lemma ref_skipI: "p \<le> q \<Longrightarrow> Spec p q \<sqsubseteq> skip"
+  by (auto simp: skip_def)
+
+lemma ref_skipE: "x \<sqsubseteq> skip \<Longrightarrow> x;y \<sqsubseteq> y"
+  by (auto simp: skip_def seq_def rel_rkat.ref_order_def)
+
+(***********************************************************************************************)
+
+text {* When using morgan, rules should be applied in the following order *}
+
+declare
+  spec_mult_isol [ref_rules]
+  spec_mult_isor [ref_rules]
+  while_iso [ref_rules]
+  leading_assignment_ref [ref_rules]
+  following_assignment_ref [ref_rules]
+  assignment_ref [ref_rules]
+  rel_rkat.skip_ref_var2 [ref_rules]
+  rel_rkat.sequence_ref [ref_rules]
+  rel_rkat.weaken_pre [ref_rules]
+  rel_rkat.strengthen_post [ref_rules]
+  rel_rkat.weaken_and_strengthen [ref_rules]
+  rel_rkat.while_ref [ref_rules]
+  while_ref_tactic [ref_rules]
+  ref_skipI [ref_rules]
+  ref_skipE [ref_rules]
+
+declare subst_def [simp]
+
+end
