HL/While.thy
@@ -1,0 +1,176 @@
+section {* While Programming Language *}
+
+theory While
+  imports Main
+begin
+
+text {* Simple while programming language based on relations *}
+
+text {* Relations below the identity form tests *}
+
+notation Id_on ("\<lfloor>_\<rfloor>" 100)
+
+text {* Variables *}
+
+text {* 
+  The following convention on types are used:
+  - 's for store, a record of variables
+  - 'a for state, the pair of 's and 'h or error state
+  - 'v for the value of a variable
+  The types are instantiated later on, and are usually generic.
+*}
+
+text {* The left value of a variable is an update function. *}
+type_synonym ('v, 's) lval = "('v \<Rightarrow> 'v) \<Rightarrow> 's \<Rightarrow> 's"
+
+text {* The right value of a variable is a retrieve function. *}
+type_synonym ('v, 's) rval = "'s \<Rightarrow> 'v"
+
+text {* A variable is then a pair of left and right values, satisfying some properties. *}
+type_synonym ('v, 's) var = "('v, 's) lval \<times> ('v, 's) rval"
+
+abbreviation upd_var :: "('v, 'a) var \<Rightarrow> ('v, 'a) lval" ("upd _" 100) where "upd_var \<equiv> fst"
+abbreviation val_var :: "('v, 'a) var \<Rightarrow> ('v, 'a) rval" ("val _" 100) where "val_var \<equiv> snd"
+
+text {* Commands *}
+
+definition abort :: "'a rel" ("abort") where "abort \<equiv> {}"
+
+definition skip :: "'a rel" ("skip") where "skip \<equiv> Id" 
+
+definition graph :: "('a \<Rightarrow> 'a) \<Rightarrow> 'a rel" ("\<langle>_\<rangle>" 100) where
+  "\<langle>f\<rangle> \<equiv> {(s, f s) | s. True}"
+
+definition subst :: "'s set \<Rightarrow> ('v, 's) lval \<Rightarrow> ('v, 's) rval \<Rightarrow> 's set" where
+  "subst P u_upd t \<equiv> Collect (\<lambda>s. (u_upd (\<lambda>_. t s) s) \<in> P)"
+
+definition assign :: "('v, 's) lval \<Rightarrow> ('s \<Rightarrow>'v) \<Rightarrow> 's rel" where
+  "assign u_upd t \<equiv> \<langle>\<lambda>s. u_upd (\<lambda>_. t s) s\<rangle>"
+
+definition seq :: "'a rel \<Rightarrow> 'a rel \<Rightarrow> 'a rel" (infixr ";" 60) where
+  "seq \<equiv> relcomp"
+
+definition cond :: "'a set \<Rightarrow> 'a rel \<Rightarrow> 'a rel \<Rightarrow> 'a rel" where
+  "cond b x y \<equiv> (Id_on b;x) \<union> (Id_on (-b);y)"
+
+definition cwhile :: "'a set \<Rightarrow> 'a rel \<Rightarrow> 'a rel" where
+  "cwhile b x \<equiv> ((Id_on b);x)\<^sup>*; (Id_on (-b))"
+
+definition cfor :: "('v :: {linorder, plus, one}, 'a) var \<Rightarrow> ('v, 'a) rval \<Rightarrow> ('v, 'a) var \<Rightarrow> 'a rel \<Rightarrow> 'a rel" where
+  "cfor j n m x \<equiv> assign (upd j) n; cwhile {s. (val j) s < (val m) s} (x; assign (upd j) (\<lambda>s. (val j) s + 1))"
+
+definition dyn :: "('a \<Rightarrow> 'a rel) \<Rightarrow> 'a rel" ("\<lceil>_\<rceil>" 100) where
+  "\<lceil>g\<rceil> \<equiv> {(\<sigma>, \<sigma>'). (\<sigma>, \<sigma>') \<in> g \<sigma>}"
+
+definition block :: "'a rel \<Rightarrow> ('a \<Rightarrow> 'a \<Rightarrow> 'a) \<Rightarrow> 'a rel" where
+  "block x ret \<equiv> \<lceil>\<lambda>\<sigma>. x; \<langle>ret \<sigma>\<rangle>\<rceil>"
+
+
+definition loc_block :: "('v, 's) var \<Rightarrow> ('v, 's) rval \<Rightarrow> 's rel \<Rightarrow> 's rel" where
+  "loc_block z t x \<equiv> (block (\<langle>\<lambda>s. (upd z) (\<lambda>_. t s) s\<rangle>; x) (\<lambda>s. (upd z) (\<lambda>_. (val z) s)))"
+
+type_synonym ('v, 'a) func = "('a rel \<times> ('v, 'a) var)"
+
+abbreviation fun_block :: "'a rel \<Rightarrow> ('v, 'a) var \<Rightarrow> ('v, 'a) func" where
+  "fun_block R y \<equiv> (R, y)"
+
+abbreviation proc_block :: "('v, 'a) func \<Rightarrow> 'a rel" ("proc _" 100) where "proc_block \<equiv> fst"
+abbreviation ret_var :: "('v, 'a) func \<Rightarrow> ('v, 'a) var" ("ret _" 100) where "ret_var \<equiv> snd"
+
+definition fun_call :: "('v, 'a) lval \<Rightarrow> ('v, 'a) func \<Rightarrow> 'a rel" where
+  "fun_call u_upd F \<equiv> let y = ret F in 
+      block (proc F) (\<lambda>s t. (upd y) (\<lambda>_. snd y s) (u_upd (\<lambda>_. snd y t) t))"
+
+text {* Annotated programs for automatic verification *}
+
+definition awhile :: "'a set \<Rightarrow> 'a set \<Rightarrow> 'a rel \<Rightarrow> 'a rel" where
+  "awhile i b x \<equiv> cwhile b x"
+
+definition afor :: "'a set \<Rightarrow> ('v :: {linorder, plus, one}, 'a) var \<Rightarrow> ('v, 'a) rval \<Rightarrow> ('v, 'a) var \<Rightarrow> 'a rel \<Rightarrow> 'a rel" where
+  "afor i j n m x \<equiv> cfor j n m x"
+
+definition apre :: "'a set \<Rightarrow> 'a rel \<Rightarrow> 'a rel" where
+  "apre p x \<equiv> x"
+
+definition apre_aux :: "('b \<Rightarrow> 'a set) \<Rightarrow> 'a rel \<Rightarrow> 'a rel" where
+  "apre_aux p x \<equiv> x"
+
+definition apost :: "'a rel \<Rightarrow> 'a set\<Rightarrow> 'a rel" where
+  "apost x q \<equiv> x; apre q skip"
+
+definition apost_aux :: "'a rel \<Rightarrow> ('b \<Rightarrow> 'a set) \<Rightarrow> 'a rel" where
+  "apost_aux x q \<equiv> x; apre_aux q skip"
+
+definition aprog :: "'a set \<Rightarrow> 'a rel \<Rightarrow> 'a set \<Rightarrow> 'a rel" where
+  "aprog p x q \<equiv> x"
+
+definition aprog_aux :: "('b \<Rightarrow> 'a set) \<Rightarrow> 'a rel \<Rightarrow> ('b \<Rightarrow> 'a set) \<Rightarrow> 'a rel" where
+  "aprog_aux p x q \<equiv> x"
+
+
+
+(***********************************************************************************************)
+
+text {* Monotonicity rules *}
+
+named_theorems mono_rules
+
+lemma mono_id [mono_rules]: "mono (\<lambda>f. f)"
+  by (auto simp: mono_def)  
+
+lemma mono_abort [mono_rules]: "mono (\<lambda>f. abort)"
+  by (auto simp: mono_def)  
+
+lemma mono_skip [mono_rules]: "mono (\<lambda>f. skip)"
+  by (auto simp: mono_def)  
+
+lemma mono_test [mono_rules]: "mono (\<lambda>f. \<lfloor>b\<rfloor>)"
+  by (auto simp: mono_def)  
+
+lemma mono_assign [mono_rules]: "mono (\<lambda>f. assign v m)"
+  by (auto simp: mono_def)  
+
+lemma mono_dyn [mono_rules]: "mono R \<Longrightarrow> mono (\<lambda>f. \<lceil>R f\<rceil>)"
+  apply (auto simp: mono_def dyn_def)
+  by (meson le_fun_def subsetCE)
+
+lemma mono_seq [mono_rules]: "mono R \<Longrightarrow> mono S \<Longrightarrow> mono (\<lambda>f. R f; S f)"
+  by (force simp: mono_def seq_def) 
+
+lemma mono_cond [mono_rules]: "mono R \<Longrightarrow> mono S \<Longrightarrow> mono (\<lambda>f. cond b (R f) (S f))"
+  by (fastforce simp: mono_def cond_def seq_def)
+
+lemma mono_iter [mono_rules]: "mono R \<Longrightarrow> mono (\<lambda>f. (R f)\<^sup>*)"
+  by (clarsimp simp: mono_def) (meson rtrancl_mono subsetCE)
+  
+lemma mono_cwhile [mono_rules]: "mono R \<Longrightarrow> mono (\<lambda>f. cwhile b (R f))"
+  by (auto simp: cwhile_def intro!: mono_rules)
+
+lemma mono_cfor [mono_rules]: "mono R \<Longrightarrow> mono (\<lambda>f. cfor j n m (R f))"
+  by (auto simp: cfor_def intro!: mono_rules)
+
+lemma mono_awhile [mono_rules]: "mono R \<Longrightarrow> mono (\<lambda>f. awhile i b (R f))"
+  by (auto simp: awhile_def intro!: mono_rules)
+
+lemma mono_afor [mono_rules]: "mono R \<Longrightarrow> mono (\<lambda>f. afor i j n m (R f))"
+  by (auto simp: afor_def intro!: mono_rules)
+
+lemma mono_apre [mono_rules]: "mono R \<Longrightarrow> mono (\<lambda>f. apre p (R f))"
+  by (auto simp: apre_def)
+
+lemma mono_apre_aux [mono_rules]: "mono R \<Longrightarrow> mono (\<lambda>f. apre_aux p (R f))"
+  by (auto simp: apre_aux_def)
+
+lemma mono_apost [mono_rules]: "mono R \<Longrightarrow> mono (\<lambda>f. apost (R f) q)"
+  by (auto simp: apost_def intro!: mono_rules)
+
+lemma mono_apost_aux [mono_rules]: "mono R \<Longrightarrow> mono (\<lambda>f. apost_aux (R f) q)"
+  by (auto simp: apost_aux_def intro!: mono_rules)
+
+lemma mono_aprog [mono_rules]: "mono R \<Longrightarrow> mono (\<lambda>f. aprog p (R f) q)"
+  by (auto simp: aprog_def)
+
+lemma mono_aprog_aux [mono_rules]: "mono R \<Longrightarrow> mono (\<lambda>f. aprog_aux p (R f) q)"
+  by (auto simp: aprog_aux_def)
+
+end
